Lambda/Lambda.v
@@ -1,9 +1,7 @@
-Require Import Coq.Unicode.Utf8.
-
-Class Lambda (A : Type) := {
-  atom : nat -> A;
-  apply : A -> A -> A;
-  abstract : nat -> A -> A;
-  complete : ∀ t : A, (∃ n : nat, t = atom n) ∨ (∃ m n : A, t = apply m n) ∨ (∃ (n : nat) (m : A), t = abstract n m);
-}.
+Module Type LambdaSig.
+  Inductive Term :=
+    | atom : nat -> Term
+    | apply : Term -> Term -> Term
+    | abstract : nat -> Term -> Term.
+End LambdaSig.
 
