Model/Seq.v
@@ -1,0 +1,39 @@
+Set Implicit Arguments.
+
+Section Seq.
+
+Variable A : Type.
+
+CoInductive Seq :=
+  | Nil : Seq
+  | Cons : A -> Seq -> Seq.
+
+Definition hd (xs : Seq) :=
+  match xs with
+  | Nil => None
+  | Cons x _ => Some x
+  end.
+
+Definition tl (xs : Seq) :=
+  match xs with
+  | Nil => None
+  | Cons _ ys => Some ys
+  end.
+
+Fixpoint nth_tl (xs : Seq) (n : nat) :=
+  match n with
+  | 0 => Some xs
+  | S m => 
+    match tl xs with
+    | None => None
+    | Some ys => nth_tl ys m
+    end
+  end.
+
+Definition nth (xs : Seq) (n : nat) :=
+  match nth_tl xs n with
+  | None => None
+  | Some ys => hd ys
+  end.
+
+End Seq.
